src/vminus/OpSemEval.v
@@ -1,0 +1,59 @@
+(** ** Evaluator for Vminus *)
+
+Require Import String.
+Require Import Vminus.Vminus.
+
+(* Some monadic set-up *)
+
+Definition err (A : Type) : Type := (string + A)%type.
+Definition err_bind {A B : Type}
+           (MA : err A) (f: A -> B) (MB : err B) :=
+  match MA with
+  | inl err => inl err
+  | inr x => inr (f x)
+  end.
+Definition err_ret {A : Type} (a : A) : err A :=
+  inr a.
+
+Notation "'do' x <- y ; z" := (err_bind y (fun x => z)) (at level 90).
+
+Module MakeEval (Import Cfg:CFG).
+
+Module SS := Make Cfg. 
+Import SS.
+
+(** *** Small-step, executable operational semantics *)
+
+Fixpoint step (g : Cfg.t) (s : state) : err state :=
+  let 'mkst mem pc loc ppc ploc := s in
+  match (fetch g pc) with
+  | Some (uid, cmd_bop bop v1 v2) =>    
+    let result := eval_bop loc bop v1 v2 in
+    match result with
+    | Some n => inr (mkst mem (incr_pc pc) (update loc uid (Some n)) ppc ploc)
+    | None => inl "cannot evalute binop command"%string
+    end 
+  | Some (uid, cmd_phi pas) =>
+    let result := eval_phi ploc (lbl_of ppc) pas in
+    match result with
+    | Some n => inr (mkst mem (incr_pc pc) (update loc uid (Some n)) ppc ploc)
+    | None => inl "cannot evaluate phi"%string
+    end
+  | Some (uid, cmd_tmn tmn) =>
+    let result := eval_tmn loc tmn in
+    match result with
+    | Some l' => inr (mkst mem (block_entry l') loc pc loc)
+    | None => inl "cannot evaluate terminator"%string
+    end
+  | Some (uid, cmd_load addr) =>
+    inr (mkst mem (incr_pc pc) (update loc uid (Some (mem addr))) ppc ploc)
+  | Some (uid, cmd_store addr v) => 
+    let result := eval_val loc v in
+    match result with
+    | Some n => inr (mkst (Memory.update mem addr n) (incr_pc pc) loc pc ploc)
+    | None => inl "cannot evaluate address to store to"%string
+    end
+  | None => inl "no instruction fetched"%string
+  end.
+
+End MakeEval.
